WIP; modify inv

security/BacktranslationProof.v
@@ -22,11 +22,18 @@ Section INVS.
              (Mem.valid_access m Mint64 b 0 Writable (Some cp)) /\
              (Mem.loadv Mint64 m (Vptr b Ptrofs.zero) (Some cp) = Some (Vlong (nat64 n))).
 
-  Definition wf_counters (ge: Clight.genv) (m: mem) (tr: bundle_trace) (cnts: cnt_ids) :=
+  Definition wf_counters (ge_a: Asm.genv) (ge: Clight.genv) (m: mem) (tr: bundle_trace) (cnts: cnt_ids) :=
     (forall id0 id1 cnt, (cnts ! id0 = Some cnt) -> (cnts ! id1 = Some cnt) -> (id0 = id1)) /\
-      (forall id b (f: function),
-          (Genv.find_symbol ge id = Some b) -> (Genv.find_funct_ptr ge b = Some (Internal f)) ->
-          (exists cnt, (cnts ! id = Some cnt) /\ (wf_counter ge m (comp_of f) (length (get_id_tr tr id)) cnt))).
+      (forall id b gd,
+          (Genv.find_symbol ge_a id = Some b) ->
+          (Genv.find_def ge_a b = Some gd) ->
+          (exists cnt, (cnts ! id = Some cnt) /\
+                    (wf_counter ge m (comp_of gd) (length (get_id_tr tr id)) cnt))).
+  (* Definition wf_counters (ge: Clight.genv) (m: mem) (tr: bundle_trace) (cnts: cnt_ids) := *)
+  (*   (forall id0 id1 cnt, (cnts ! id0 = Some cnt) -> (cnts ! id1 = Some cnt) -> (id0 = id1)) /\ *)
+  (*     (forall id b (f: function), *)
+  (*         (Genv.find_symbol ge id = Some b) -> (Genv.find_funct_ptr ge b = Some (Internal f)) -> *)
+  (*         (exists cnt, (cnts ! id = Some cnt) /\ (wf_counter ge m (comp_of f) (length (get_id_tr tr id)) cnt))). *)
 
   Inductive wf_c_cont (ge: Clight.genv) : mem -> cont -> Prop :=
   | wf_c_cont_nil
@@ -59,6 +66,15 @@ Section INVS.
           (wf_env ge e /\ (not_global_blks (ge) (blocks_of_env2 ge e)) /\ (wf_c_nb ge m_c))
     | _ => False
     end.
+  (* Definition wf_c_state (ge: Clight.genv) (tr ttr: bundle_trace) (cnts: cnt_ids) id (cst: Clight.state) := *)
+  (*   match cst with *)
+  (*   | State f stmt k_c e le m_c => *)
+  (*       wf_counters ge m_c tr cnts /\ *)
+  (*         (exists m_c', Mem.free_list m_c (blocks_of_env ge e) (comp_of f) = Some m_c' /\ wf_c_cont ge m_c' k_c) /\ *)
+  (*         wf_c_stmt ge (comp_of f) cnts id ttr stmt /\ *)
+  (*         (wf_env ge e /\ (not_global_blks (ge) (blocks_of_env2 ge e)) /\ (wf_c_nb ge m_c)) *)
+  (*   | _ => False *)
+  (*   end. *)
 
   Definition match_genv (ge: Asm.genv) (ge': genv) :=
     (match_symbs ge ge') /\ (eq_policy ge ge').
